symbolic augmentation of recursive cases in function summation

CaseStudy/K3.lean
@@ -1,8 +1,9 @@
 --
 -- Kleene K3 logic (logic of indeterminacy)
 --
-import AR.Tools.Compose
-import Lean
+import LeanToolkit
+
+set_option pp.fieldNotation.generalized false
 
 --class TermOps (α: Type) where
 --  countNodes : α → Nat
@@ -19,18 +20,12 @@ def countNodes (t: Term): Nat :=
 | .T => 1
 | .F => 1
 
-#check countNodes.eq_unfold
-
 theorem positiveSize: ∀x: Term, countNodes x > 0 :=
 by intros x; cases x <;> simp[countNodes]
 
---instance (α: Σ T, TermOps T): TermOps (BTerm α) where
---  countNodes := _countNodes α
---  positiveSize := _positiveSize α
-
 end Boolean
 
-/-
+
 namespace Indet
 
 inductive Term
@@ -40,10 +35,9 @@ def countNodes(t: Term): Nat :=
 1+ match t with
 | .I => 1
 
-theorem eq (t: Term): t = t := by rfl
+theorem positiveSize (t: Term): countNodes t > 0  := by simp[countNodes]
 
 end Indet
--/
 
 namespace Ops
 
@@ -68,171 +62,178 @@ by
   | Or x y  => simp[countNodes]; rw [Nat.one_add, Nat.succ_add]; simp[Nat.zero_lt_succ]
   | Imp x y => simp[countNodes]; rw [Nat.one_add, Nat.succ_add]; simp[Nat.zero_lt_succ]
 
-#print positiveSize
---instance TTOps (α: Σ T, TermOps T): TermOps (Term α) where
---  countNodes := _countNodes α
---  positiveSize := _positiveSize α
-
 end Ops
 
-namespace BooleanLogic
+--namespace BooleanLogic
 inductive Term := Boolean.Term |+ Ops.Term
-#print Term
-
-def countNodes(t: Term): Nat :=
-  match t with
-  | .T        => 1
-  | .F        => 1
-  | .Neg t    => 1 + (countNodes t)
-  | .And t₁ t₂  => 1 + countNodes t₁ + countNodes t₂
-  | .Or t₁ t₂   => 1 + countNodes t₁ + countNodes t₂
-  | .Imp t₁ t₂  => 1 + countNodes t₁ + (countNodes t₂)
-
-#print Ops.countNodes.eq_unfold
---theorem positiveSize: ∀x: Term, countNodes x > 0 :=
---by
---  intros x; cases x <;> first | try apply Boolean.positiveSize | try apply Ops.positiveSize
-/-
-  intros x
-  induction x with
-  | T => simp[countNodes]
-  | F => simp[countNodes]
-  | Neg x   => simp[countNodes]; rw [Nat.one_add]; simp[Nat.zero_lt_succ]
-  | And x y => simp[countNodes]; rw [Nat.one_add, Nat.succ_add]; simp[Nat.zero_lt_succ]
-  | Or x y  => simp[countNodes]; rw [Nat.one_add, Nat.succ_add]; simp[Nat.zero_lt_succ]
-  | Imp x y ih₁ ih₂ => simp[countNodes]; apply Nat.lt_add_left; exact ih₂
+/--
+info:
+inductive Term : Type
+number of parameters: 0
+constructors:
+Term.T : Term
+Term.F : Term
+Term.Neg : Term → Term
+Term.And : Term → Term → Term
+Term.Or : Term → Term → Term
+Term.Imp : Term → Term → Term
 -/
-/-
-def countNodes: Term → Nat
-| Term.T => Boolean.countNodes Term.T
-| Term.F => Boolean.countNodes Term.F
-| Term.I => Indet.countNodes Term.I
--/
-
-
-/-
-fn countNodes := Boolean.countNodes + Indet.countNodes + Ops.countNodes
+#guard_msgs in
 #print Term
-def countNodes (t: Term):  Nat :=
-  match t with
-  | .T => Boolean.countNodes .T
-  | .F => Boolean.countNodes .F
-  | .I => Indet.countNodes .I
-  | .Neg t => countNodes_Ops (.Neg t) --Term → Term
-where
-  countNodes_Ops (t: Term) :=
-  match t with
-  | .Neg t      => 1 + countNodes t
-  | .And t₁ t₂  => 1 + countNodes t₁ + countNodes t₂
-  | .Or t₁ t₂   => 1 + countNodes t₁ + countNodes t₂
-  | .Imp t₁ t₂  => 1 + countNodes t₁ + countNodes t₂
-  -/
---Term.And : Term → Term → Term
---Term.Or : Term → Term → Term
---Term.Imp : Term → Term → Term
 
---theorem eq (t: Term): t = t := Boolean.eq
---by
---  cases t with --first | apply Boolean.eq | apply Indet.eq | apply Ops.eq
---  | T => apply Boolean.eq ↑.T
---  | F => apply Boolean.eq
---  | I => apply Indet.eq
-
- --<;> first | apply Boolean.eq | apply Indet.eq | apply Ops.eq
-
---inductive countNodes := Boolean.countNodes + Indet.countNodes
---| .T => Boolean.countNodes .T
---| .F => Boolean.countNodes .F
---| .I => Indet.countNodes .I
---| .Neg t => Ops.countNodes (.Neg t)
-
-
-
---<;> Boolean.countNodes | Ops.countNodes
-
---| .T => countNodes .T
-
---BooleanLogic.Term.F : Term
---BooleanLogic.Term.Neg : Term → Term
---BooleanLogic.Term.And : Term → Term → Term
---BooleanLogic.Term.Or : Term → Term → Term
---BooleanLogic.Term.Imp : Term → Term → Term
-end BooleanLogic
-
-namespace K3Logic
-
-inductive Term := Boolean.Term |+ Indet.Term |+ Ops.Term
-#print Term
-end K3Logic
-
-namespace baseline
-inductive Term
-| T | F | I
-| Neg (t: Term)
-| And (t₁ t₂: Term)
-| Or  (t₁ t₂: Term)
-| Imp (t₁ t₂: Term)
-
-def countNodes: Term→ Nat
-| .T          => 1
-| .F          => 1
-| .I          => 1
-| .Neg t      => 1 + countNodes t
+fn countNodes: Term → Nat := Boolean.countNodes |+ Ops.countNodes
+| .Neg t    => 1 + (countNodes t)
 | .And t₁ t₂  => 1 + countNodes t₁ + countNodes t₂
 | .Or t₁ t₂   => 1 + countNodes t₁ + countNodes t₂
-| .Imp t₁ t₂  => 1 + countNodes t₁ + countNodes t₂
+| .Imp t₁ t₂  => 1 + countNodes t₁ + (countNodes t₂)
 
-namespace Boolean
-
-inductive Term
-| T
-| F
-
-def countNodes: Term→ Nat
-| .T          => 1
-| .F          => 1
-
-end Boolean
-
-namespace Indet
-
-inductive Term
-| I
-
-def countNodes: Term → Nat
-| .I          => 1
-
-end Indet
-
-namespace Ops
-
-inductive Term
-| Neg (t: Term)
-| And (t₁ t₂: Term)
-| Or  (t₁ t₂: Term)
-| Imp (t₁ t₂: Term)
-
-def countNodes: Term→ Nat
-| .Neg t      => 1 + countNodes t
-| .And t₁ t₂  => 1 + countNodes t₁ + countNodes t₂
-| .Or t₁ t₂   => 1 + countNodes t₁ + countNodes t₂
-| .Imp t₁ t₂  => 1 + countNodes t₁ + countNodes t₂
-
-end Ops
---
--- def Lean.Meta.getConstUnfoldEqnFor? (declName : Name) :
---MetaM (Option Name)
-
---Returns the "const unfold" theorem (f.eq_unfold) for the given declaration. This is not extensible, and always builds on the unfold theorem (f.eq_def).
-
-#check countNodes.eq_unfold
-def x := Term.T
-#print x
-
-#check Term.brecOn
-#check Term.below
-#print Term.below
-#check Term.rec
-
+/--
+info:
+def countNodes : Term → Nat :=
+fun x =>
+  Term.brecOn x fun x f =>
+    (match (motive := (x : Term) → Term.below x → Nat) x with
+      | Term.T => fun x => Boolean.countNodes Boolean.Term.T
+      | Term.F => fun x => Boolean.countNodes Boolean.Term.F
+      | Term.Neg t => fun x => 1 + x.1
+      | Term.And t₁ t₂ => fun x => 1 + x.1.1 + x.2.1
+      | Term.Or t₁ t₂ => fun x => 1 + x.1.1 + x.2.1
+      | Term.Imp t₁ t₂ => fun x => 1 + x.1.1 + x.2.1)
+      f
+-/
+#guard_msgs in
 #print countNodes
-end baseline
+
+fn positiveSize(x: Term): countNodes x > 0 := Boolean.positiveSize |+ Ops.positiveSize
+| .Neg x   => by simp[countNodes]; rw [Nat.one_add]; simp[Nat.zero_lt_succ]
+| .And x y => by simp[countNodes]; rw [Nat.one_add, Nat.succ_add]; simp[Nat.zero_lt_succ]
+| .Or x y  => by simp[countNodes]; rw [Nat.one_add, Nat.succ_add]; simp[Nat.zero_lt_succ]
+| .Imp x y => by simp[countNodes]; rw [Nat.one_add, Nat.succ_add]; simp[Nat.zero_lt_succ]
+
+/--
+info:
+def positiveSize : ∀ (x : Term), countNodes x > 0 :=
+fun x =>
+  match x with
+  | Term.T => Boolean.positiveSize Boolean.Term.T
+  | Term.F => Boolean.positiveSize Boolean.Term.F
+  | Term.Neg x =>
+    Eq.mpr (id gt_iff_lt._simp_1)
+      (Eq.mpr (id (congrArg (fun _a => 0 < _a) (Nat.one_add (countNodes x))))
+        (of_eq_true (Nat.zero_lt_succ._simp_1 (countNodes x))))
+  | Term.And x y =>
+    Eq.mpr (id gt_iff_lt._simp_1)
+      (Eq.mpr (id (congrArg (fun _a => 0 < _a + countNodes y) (Nat.one_add (countNodes x))))
+        (Eq.mpr (id (congrArg (fun _a => 0 < _a) (Nat.succ_add (countNodes x) (countNodes y))))
+          (of_eq_true (Nat.zero_lt_succ._simp_1 (countNodes x + countNodes y)))))
+  | Term.Or x y =>
+    Eq.mpr (id gt_iff_lt._simp_1)
+      (Eq.mpr (id (congrArg (fun _a => 0 < _a + countNodes y) (Nat.one_add (countNodes x))))
+        (Eq.mpr (id (congrArg (fun _a => 0 < _a) (Nat.succ_add (countNodes x) (countNodes y))))
+          (of_eq_true (Nat.zero_lt_succ._simp_1 (countNodes x + countNodes y)))))
+  | Term.Imp x y =>
+    Eq.mpr (id gt_iff_lt._simp_1)
+      (Eq.mpr (id (congrArg (fun _a => 0 < _a + countNodes y) (Nat.one_add (countNodes x))))
+        (Eq.mpr (id (congrArg (fun _a => 0 < _a) (Nat.succ_add (countNodes x) (countNodes y))))
+          (of_eq_true (Nat.zero_lt_succ._simp_1 (countNodes x + countNodes y)))))
+-/
+#guard_msgs in
+#print positiveSize
+
+inductive K3Term := Boolean.Term |+ Indet.Term |+ Ops.Term
+
+/--
+info:
+inductive K3Term : Type
+number of parameters: 0
+constructors:
+K3Term.T : K3Term
+K3Term.F : K3Term
+K3Term.I : K3Term
+K3Term.Neg : K3Term → K3Term
+K3Term.And : K3Term → K3Term → K3Term
+K3Term.Or : K3Term → K3Term → K3Term
+K3Term.Imp : K3Term → K3Term → K3Term
+-/
+#guard_msgs in
+#print K3Term
+
+fn K3countNodes: K3Term → Nat := Boolean.countNodes |+ Indet.countNodes |+ Ops.countNodes
+| .Neg t    => 1 + (K3countNodes t)
+| .And t₁ t₂  => 1 + K3countNodes t₁ + K3countNodes t₂
+| .Or t₁ t₂   => 1 + K3countNodes t₁ + K3countNodes t₂
+| .Imp t₁ t₂  => 1 + K3countNodes t₁ + (K3countNodes t₂)
+
+/--
+info:
+def K3countNodes : K3Term → Nat :=
+fun x =>
+  K3Term.brecOn x fun x f =>
+    (match (motive := (x : K3Term) → K3Term.below x → Nat) x with
+      | K3Term.T => fun x => Boolean.countNodes Boolean.Term.T
+      | K3Term.F => fun x => Boolean.countNodes Boolean.Term.F
+      | K3Term.I => fun x => Indet.countNodes Indet.Term.I
+      | K3Term.Neg t => fun x => 1 + x.1
+      | K3Term.And t₁ t₂ => fun x => 1 + x.1.1 + x.2.1
+      | K3Term.Or t₁ t₂ => fun x => 1 + x.1.1 + x.2.1
+      | K3Term.Imp t₁ t₂ => fun x => 1 + x.1.1 + x.2.1)
+      f
+-/
+#guard_msgs in
+#print K3countNodes
+
+fnRec K3countNodes': K3Term → Nat := Boolean.countNodes |+ Indet.countNodes |+ Ops.countNodes
+
+/--
+info:
+def K3countNodes' : K3Term → Nat :=
+fun x =>
+  K3Term.brecOn x fun x f =>
+    (match (motive := (x : K3Term) → K3Term.below x → Nat) x with
+      | K3Term.T => fun x => Boolean.countNodes Boolean.Term.T
+      | K3Term.F => fun x => Boolean.countNodes Boolean.Term.F
+      | K3Term.I => fun x => Indet.countNodes Indet.Term.I
+      | K3Term.Neg t => fun x => 1 + x.1
+      | K3Term.And t₁ t₂ => fun x => 1 + x.1.1 + x.2.1
+      | K3Term.Or t₁ t₂ => fun x => 1 + x.1.1 + x.2.1
+      | K3Term.Imp t₁ t₂ => fun x => 1 + x.1.1 + x.2.1)
+      f
+-/
+#guard_msgs in
+#print K3countNodes'
+
+fn K3positiveSize(x: Term): countNodes x > 0 := Boolean.positiveSize |+ Indet.positiveSize |+ Ops.positiveSize
+| .Neg x   => by simp[countNodes]; rw [Nat.one_add]; simp[Nat.zero_lt_succ]
+| .And x y => by simp[countNodes]; rw [Nat.one_add, Nat.succ_add]; simp[Nat.zero_lt_succ]
+| .Or x y  => by simp[countNodes]; rw [Nat.one_add, Nat.succ_add]; simp[Nat.zero_lt_succ]
+| .Imp x y => by simp[countNodes]; rw [Nat.one_add, Nat.succ_add]; simp[Nat.zero_lt_succ]
+
+/--
+info:
+def K3positiveSize : ∀ (x : Term), countNodes x > 0 :=
+fun x =>
+  match x with
+  | Term.T => Boolean.positiveSize Boolean.Term.T
+  | Term.F => Boolean.positiveSize Boolean.Term.F
+  | Term.Neg x =>
+    Eq.mpr (id gt_iff_lt._simp_1)
+      (Eq.mpr (id (congrArg (fun _a => 0 < _a) (Nat.one_add (countNodes x))))
+        (of_eq_true (Nat.zero_lt_succ._simp_1 (countNodes x))))
+  | Term.And x y =>
+    Eq.mpr (id gt_iff_lt._simp_1)
+      (Eq.mpr (id (congrArg (fun _a => 0 < _a + countNodes y) (Nat.one_add (countNodes x))))
+        (Eq.mpr (id (congrArg (fun _a => 0 < _a) (Nat.succ_add (countNodes x) (countNodes y))))
+          (of_eq_true (Nat.zero_lt_succ._simp_1 (countNodes x + countNodes y)))))
+  | Term.Or x y =>
+    Eq.mpr (id gt_iff_lt._simp_1)
+      (Eq.mpr (id (congrArg (fun _a => 0 < _a + countNodes y) (Nat.one_add (countNodes x))))
+        (Eq.mpr (id (congrArg (fun _a => 0 < _a) (Nat.succ_add (countNodes x) (countNodes y))))
+          (of_eq_true (Nat.zero_lt_succ._simp_1 (countNodes x + countNodes y)))))
+  | Term.Imp x y =>
+    Eq.mpr (id gt_iff_lt._simp_1)
+      (Eq.mpr (id (congrArg (fun _a => 0 < _a + countNodes y) (Nat.one_add (countNodes x))))
+        (Eq.mpr (id (congrArg (fun _a => 0 < _a) (Nat.succ_add (countNodes x) (countNodes y))))
+          (of_eq_true (Nat.zero_lt_succ._simp_1 (countNodes x + countNodes y)))))
+-/
+#guard_msgs in
+#print K3positiveSize
