LeanToolkit/TypeSum.lean
@@ -73,7 +73,7 @@ private def checkTypeCompat
           then return e
           else throwError m!"{t} and {e} are different types."
 
-def concatConstructors
+private def concatConstructors
   (css: List (List TracedConstructor))
 : TermElabM (List TracedConstructor) := do
   match css with
@@ -158,30 +158,6 @@ declare_syntax_cat types
 syntax (name := singleton) ident: types
 syntax (name := typeSum) types " |+ " types : types
 
---
--- create a new hidden inductive type with the explicit constructors
--- then append the name of the created type to the list of types to
--- be summed up
---
-private def includeExplicitConstructors
-  (d: Ident)
-  (sig: TSyntax `Lean.Parser.Command.optDeclSig)
-  (cs : TSyntax `types)
-  (explicitCs: TSyntaxArray `Lean.Parser.Command.ctor): CommandElabM (TSyntax `types)
-:= do
-  let hiddenName := Name.append (Name.mkStr1 "hidden") d.getId
-  let ⟨_, s⟩  := expandOptDeclSig sig
-  -- logInfo m!"sig - {sig} - {s}"
-  let hiddenSig:TSyntax `Lean.Parser.Command.optDeclSig ←
-    if s.isSome then pure sig else `(optDeclSig| : Type)
-
-  let cmd ← `(inductive $d $hiddenSig where $explicitCs:ctor*)
-  -- logInfo m!"hidden command: {cmd}"
-
-  withNamespace (Name.mkStr1 "hidden") (elabCommand cmd)
-
-  `(types| $cs |+ $(mkIdent hiddenName):ident)
-
 /-
   resolveTypeName
 
@@ -216,7 +192,6 @@ private partial def getTypeVals': TSyntax `types → TermElabM (List Name)
 | _ => return  []
 
 def getTypeVals(cs: TSyntax `types): TermElabM (List InductiveVal) := do
-  --let env ← getEnv
   let ns ← getTypeVals' cs
   let ns' := List.eraseDups ns
   ns'.mapM getInductiveVal
@@ -225,19 +200,13 @@ def getTypeVals(cs: TSyntax `types): TermElabM (List InductiveVal) := do
 --  elaborator for type sum syntax
 --
 elab "inductive " d:ident sig':optDeclSig " := " cs':types explicitCs: ctor* : command => do
-  --let ns ← getCurrNamespace
-  --let ns := if ns'.isAnonymous then `_root_ else ns'
-  --logInfo m!"ns: {ns}"
-  --withNamespace ns do
   let mut cs := cs'
-  let lhs := /-ns.append-/ d.getId
-  --logInfo m!"lhs: {lhs}"
+  let lhs := d.getId
 
   let (_, optSig) := expandOptDeclSig sig'
   let expectedType ← optSig.bindM
     (λ s ↦ do pure <| some (← liftTermElabM <| elabType s))
 
-  --logInfo m!"expected type: {expectedType}"
   let ts ← liftTermElabM <| getTypeVals cs
 
   let ⟨cObjs, e, _⟩ ← liftTermElabM <| typeSumImp ts expectedType lhs
@@ -251,23 +220,10 @@ elab "inductive " d:ident sig':optDeclSig " := " cs':types explicitCs: ctor* : c
   let cStx := cStx.toArray ++ explicitCs
   let e' ← liftTermElabM <| PrettyPrinter.delab e
   let cmd ← `(inductive $(mkIdent lhs) : $e' $cStx:ctor*)
-  --logInfo m!"elaborating {cmd}"
   elabCommand cmd
 
-  -- add supertype record to environment extension
   liftTermElabM <| addSuperType (Expr.const lhs []) cObjs
 
-  --let ns ← getCurrNamespace
-  --let ns := if ns'.isAnonymous then `_root_ else ns'
-  --logInfo m!"ns: {ns}"
-  --withNamespace ns do
-  --let mut cs := cs'
-  --let lhs := /-ns.append-/ d.getId
-  --let s ← liftTermElabM <| getInductiveVal lhs
   let propType ← liftTermElabM <| isPropFormerType e --s.type
   if !propType then
     genCoeInst lhs e cObjs
-    --for t in ts do
-      --let t ← liftTermElabM <| getInductiveVal t.name
-      --upCoe s t
-      --downCoe t s
